pulse/examples/dsls/mini_steel/Pulse.Soundness.fst
@@ -14,16 +14,7 @@ module Frame = Pulse.Soundness.Frame
 module STEquiv = Pulse.Soundness.STEquiv
 module Return = Pulse.Soundness.Return
 
-assume
-val equiv_beta (g:R.env) 
-               (x:R.var)
-               (ty:R.term { RT.lookup_bvar g x == Some ty })
-               (t:R.term {RT.ln' t 0})
-  : GTot (RT.equiv g t
-                     (R.mk_app (mk_abs ty (RT.close_term t x))
-                               [mk_name x, R.Q_Explicit]))
 
-    
 #push-options "--query_stats --fuel 2 --ifuel 2 --z3rlimit_factor 10"
 let rec soundness (f:stt_env)
                   (g:env)
@@ -34,6 +25,7 @@ let rec soundness (f:stt_env)
          (decreases d)
   = let mk_t_abs (#u:universe)
                  (#ty:pure_term)
+                 (q:option qualifier)
                  (ppname:string)
                  (t_typing:tot_typing f g ty (Tm_Type u) { t_typing << d })
                  (#body:term)
@@ -41,8 +33,8 @@ let rec soundness (f:stt_env)
                  (#c:pure_comp)
                  (body_typing:src_typing f ((x, Inl ty)::g) (open_term body x) c { body_typing << d })
       : GTot (RT.typing (extend_env_l f g)
-                        (mk_abs_with_name ppname (elab_pure ty) (RT.close_term (elab_src_typing body_typing) x))
-                        (elab_pure (Tm_Arrow {binder_ty=ty;binder_ppname=ppname} (close_pure_comp c x))))
+                        (mk_abs_with_name ppname (elab_pure ty) (elab_qual q) (RT.close_term (elab_src_typing body_typing) x))
+                        (elab_pure (Tm_Arrow {binder_ty=ty;binder_ppname=ppname} q (close_pure_comp c x))))
       = let E t_typing = t_typing in
         let r_t_typing = soundness _ _ _ _ t_typing in
         let r_body_typing = soundness _ _ _ _ body_typing in
@@ -51,21 +43,22 @@ let rec soundness (f:stt_env)
     match d with
     | T_Tot _ _ _ d -> d
 
-    | T_Abs _ ppname x ty u body c hint _ t_typing body_typing ->
-      mk_t_abs ppname t_typing body_typing    
+    | T_Abs _ ppname x q ty u body c hint _ t_typing body_typing ->
+      mk_t_abs q ppname t_typing body_typing    
 
-    | T_STApp _ head ppname formal res arg head_typing arg_typing ->
+
+    | T_STApp _ head ppname formal q res arg head_typing arg_typing ->
       let E arg_typing = arg_typing in
       let r_head = elab_src_typing head_typing in
       let r_arg = elab_pure arg in
       elab_pure_equiv arg_typing;
       let r_head_typing
-        : RT.typing _ r_head (elab_pure (Tm_Arrow {binder_ty=formal;binder_ppname=ppname} res))
+        : RT.typing _ r_head (elab_pure (Tm_Arrow {binder_ty=formal;binder_ppname=ppname} q res))
         = soundness _ _ _ _ head_typing
       in
       let r_arg_typing = soundness _ _ _ _ arg_typing in
       elab_comp_open_commute res arg;
-      RT.T_App _ _ _ (binder_of_t_q_s (elab_pure formal) R.Q_Explicit ppname)
+      RT.T_App _ _ _ (binder_of_t_q_s (elab_pure formal) (elab_qual q) ppname)
                      (elab_pure_comp res)
                      r_head_typing
                      r_arg_typing
@@ -76,8 +69,8 @@ let rec soundness (f:stt_env)
         = soundness _ _ _ _ e1_typing
       in
       let r2_typing
-        : RT.typing _ _ (elab_pure (Tm_Arrow (null_binder (comp_res c1)) (close_pure_comp c2 x)))
-        = mk_t_abs _ t_typing e2_typing
+        : RT.typing _ _ (elab_pure (Tm_Arrow (null_binder (comp_res c1)) None (close_pure_comp c2 x)))
+        = mk_t_abs None _ t_typing e2_typing
       in
       let Bind_comp _ _ _ _ t2_typing y post2_typing = bc in
       assume (~ (x `Set.mem` freevars_comp c1));
